theories/soundness.v
@@ -10,3 +10,6 @@ Theorem fundamental_theorem :
   apply wt_mutual; eauto with sem; [hauto l:on use:SE_Pair].
   Unshelve. all : exact 0.
 Qed.
+
+Lemma synsub_to_usub : forall n Γ (a b : PTm n), Γ ⊢ a ≲ b -> SN a /\ SN b /\ Sub.R a b.
+Proof. hauto lq:on rew:off use:fundamental_theorem, SemLEq_SN_Sub. Qed.
